vale/code/crypto/aes/AES_helpers.fsti
@@ -111,18 +111,13 @@ val finish_cipher (alg:algorithm) (input:quad32) (round_keys:seq quad32) :
             let state = quad32_xor state (index round_keys (nr alg)) in
             state == cipher_opaque alg input round_keys))
 
-(*
-val finish_cipher_opt (alg:algorithm) (input plain:quad32) (round_keys:seq quad32) :
-  Lemma
-    (length round_keys == (nr alg) + 1 ==>
-        length round_keys > 0 /\ nr alg > 1 /\   // REVIEW: Why are these needed?
-           (let state = quad32_xor input (index round_keys 0) in
-            let state = rounds_opaque state round_keys (nr alg - 1) in
-            let state = shift_rows_LE state in
-            let state = sub_bytes state in
-            let state = quad32_xor state (quad32_xor plain (index round_keys (nr alg))) in
-            state == quad32_xor plain (cipher_opaque alg input round_keys)))
-*)
+val finish_cipher_opt (alg:algorithm) (input plain t0 t1 out:quad32) (round_keys:seq quad32) : Lemma
+  (requires length round_keys == (nr alg) + 1 /\
+            length round_keys > 0 /\ nr alg > 1 /\   // REVIEW: Why are these needed?
+            t0 = quad32_xor input (index round_keys 0) /\
+            t1 = rounds_opaque t0 round_keys (nr alg - 1) /\
+            out = quad32_xor (sub_bytes (shift_rows_LE t1)) (quad32_xor plain (index round_keys (nr alg))))
+  (ensures out == quad32_xor plain (cipher_opaque alg input round_keys))
 
 
 val lemma_incr_msb (orig ctr ctr':quad32) (increment:nat) : Lemma
